axiomatic_expressions.v
@@ -22,11 +22,15 @@ Implicit Types k : ctx K.
 Implicit Types φ : focus K.
 Implicit Types S : state K.
 
+Arguments assert_holds _ _ _ _ _ _ _ _ : simpl never.
+
 Hint Extern 1 (_ ⊥ _) => solve_mem_disjoint.
 Hint Extern 1 (⊥ _) => solve_mem_disjoint.
 Hint Extern 1 (sep_valid _) => solve_mem_disjoint.
 Hint Extern 1 (_ ≤ _) => omega.
 
+Hint Resolve Forall_app_2.
+Hint Immediate memenv_subseteq_forward.
 Hint Immediate cmap_valid_memenv_valid.
 Hint Resolve cmap_empty_valid cmap_erased_empty mem_locks_empty.
 Hint Resolve cmap_union_valid_2 cmap_erased_union cmap_erase_valid.
@@ -170,8 +174,9 @@ Proof.
           eauto 3 using cmap_erased_subseteq, @sep_union_subseteq_r'.
         by rewrite <-!(sep_associative m'),
           (sep_commutative mA mf), !sep_associative by auto.
-      - destruct (λ H, IH n' H Δ'' ρ [] φ' m' τlr); eauto using
-          indexes_valid_weaken, cmap_erased_subseteq, @sep_union_subseteq_l'.
+      - destruct (λ H, IH n' H Δ'' ρ [] φ' m' τlr); eauto 10 using
+          indexes_valid_weaken, cmap_erased_subseteq, @sep_union_subseteq_l',
+          assert_weaken.
     + apply mk_ax_next with Δ'' m'; auto; [by apply ax_unframe_fun_to_fun|].
       destruct (λ H, IH n' H Δ'' ρ k' φ' m' τlr);
         eauto using indexes_valid_weaken.
@@ -253,7 +258,8 @@ Proof.
   intros Δ' n' ????? Hframe; inversion_clear Hframe as [mA mf|];
     simplify_equality; simplify_mem_disjoint_hyps.
   destruct (HQ Γ' Δ ρ n (cmap_erase m)) as [? HA]; eauto.
-  destruct (HA Γ' Δ' n' mA) as (τlr&_&?); clear HA; eauto.
+  destruct (HA Γ' Δ' n' mA) as (τlr&_&?); clear HA;
+    eauto 4 using assert_weaken, indexes_valid_weaken.
   { rewrite <-cmap_erase_disjoint_le; auto. }
   simplify_option_equality. typed_inversion_all.
   split; [solve_rcred|intros ? p _].
@@ -270,15 +276,16 @@ Lemma ax_rtol Γ δ A P Q1 Q2 e :
   Γ\ δ\ A ⊨ₑ {{ P }} .* e {{ Q2 }}.
 Proof.
   intros HQ Hax Γ' Δ n ρ m [τ|] ????? He1e2 He ???; typed_inversion_all.
-  apply (ax_expr_compose_1 Γ' δ A Q1 _ Δ DCRtoL e ρ n m (inr (TType τ.*))); auto.
+  apply (ax_expr_compose_1 Γ' δ A Q1 _ Δ DCRtoL e ρ n m (inr (TType τ.* ))); auto.
   { esolve_elem_of. }
-  clear dependent m; intros Δ' n' Ω [|v] m ??????; typed_inversion_all.
+  clear dependent m; intros Δ' n' [|v] m ?????; typed_inversion_all.
   apply ax_further_alt.
   intros Δ'' n'' ????? Hframe; inversion_clear Hframe as [mA mf|];
     simplify_equality; simplify_mem_disjoint_hyps.
   destruct (HQ v Γ' Δ' ρ n' (cmap_erase m)) as (a'&?&HA);
     simpl; eauto 10 using indexes_valid_weaken.
-  destruct (HA Γ' Δ'' n'' mA) as (τlr&?&?); clear HA; eauto.
+  destruct (HA Γ' Δ'' n'' mA) as (τlr&?&?); clear HA;
+    eauto 4 using assert_weaken, indexes_valid_weaken.
   { rewrite <-cmap_erase_disjoint_le; auto. }
   destruct τlr as [τ'|]; simplify_option_equality; typed_inversion_all.
   assert (TType τ' = TType τ); [|simplify_equality].
@@ -304,7 +311,7 @@ Proof.
   intros HQ Hax Γ' Δ n ρ m [τ|] ????? He1e2 He ???; typed_inversion_all.
   apply (ax_expr_compose_1 Γ' δ A Q1 _ Δ DCRofL e ρ n m (inl τ)); auto.
   { esolve_elem_of. }
-  clear dependent m; intros Δ' n' Ω [a|] m ??????; typed_inversion_all.
+  clear dependent m; intros Δ' n' [a|] m ?????; typed_inversion_all.
   apply ax_further; [intros; solve_rcred|].
   intros Δ'' n'' ?? S' ??? Hframe p _; inversion_clear Hframe as [mA mf|];
     simplify_equality; simplify_mem_disjoint_hyps.
@@ -323,14 +330,15 @@ Proof.
   intros HQ Hax Γ' Δ n ρ m [|τ] ???????? HA HP; typed_inversion_all.
   apply (ax_expr_compose_1 Γ' δ A Q1 _ Δ DCLoad e ρ n m (inl τ)); auto.
   { esolve_elem_of. }
-  clear dependent m. intros Δ' n' Ω [a|] m ??????; typed_inversion_all.
+  clear dependent m. intros Δ' n' [a|] m ?????; typed_inversion_all.
   apply ax_further_alt; intros Δ'' n'' ????? Hframe;
     inversion_clear Hframe as [mA mf|]; simplify_equality.
   destruct (HQ a Γ' Δ' ρ n' (cmap_erase m))
     as (v&?&HA); eauto using indexes_valid_weaken.
   assert (⊥ [mA; cmap_erase m]).
   { rewrite <-cmap_erase_disjoint_le; auto. }
-  destruct (HA Γ' Δ'' n'' mA) as (τlr&?&?); clear HA; eauto.
+  destruct (HA Γ' Δ'' n'' mA) as (τlr&?&?); clear HA;
+    eauto 4 using assert_weaken, indexes_valid_weaken.
   destruct τlr as [|τ']; simplify_option_equality; typed_inversion_all.
   assert (mA ∪ cmap_erase m ⊆ m ∪ mf ∪ mA).
   { rewrite (sep_commutative _ mA) by auto.
@@ -386,8 +394,8 @@ Proof.
     @sep_union_subseteq_l', @sep_union_subseteq_r'.
   { esolve_elem_of. }
   { esolve_elem_of. }
-  clear dependent m1 m2; intros Δ' n' Ω1 Ω2 [a'|] [|v] m1' m2'
-    ???????????; typed_inversion_all.
+  clear dependent m1 m2; intros Δ' n' [a'|] [|v] m1' m2'
+    ?????????; typed_inversion_all.
   apply ax_further_alt; intros Δ'' n'' ? ff ??? Hframe;
     inversion_clear Hframe as [mA mf|]; simplify_equality.
   destruct (HQ a' v Γ' Δ' ρ n' (cmap_erase (m1' ∪ m2')))
@@ -416,7 +424,8 @@ Proof.
     { rewrite <-cmap_erase_disjoint_le; auto. }
     eapply assign_sem_subseteq with Δ'' (mA ∪ cmap_erase (m1 ∪ m2)) τ1 τ2;
       eauto 15 using addr_typed_weaken, val_typed_weaken.
-    destruct ass; destruct (Hass Γ' Δ'' n'' mA) as [(?&_&?) (?&_&?)]; auto;
+    destruct ass; destruct (Hass Γ' Δ'' n'' mA) as [(?&_&?) (?&_&?)];
+      eauto 4 using assert_weaken, indexes_valid_weaken;
       clear Hass; simplify_option_equality;
       econstructor; simplify_type_equality; eauto. }
   clear Hass.
@@ -473,13 +482,14 @@ Proof.
     by (typed_inversion_all; eauto); clear He.
   apply (ax_expr_compose_1 Γ' δ A Q1 _ Δ (DCEltL rs) e ρ n m (inl τ)); auto.
   { esolve_elem_of. }
-  clear dependent m; intros Δ' n' Ω [a|] m ??????; typed_inversion_all.
+  clear dependent m; intros Δ' n' [a|] m ?????; typed_inversion_all.
   apply ax_further_alt.
   intros Δ'' n'' ????? Hframe; inversion_clear Hframe as [mA mf|];
     simplify_equality; simplify_mem_disjoint_hyps.
   destruct (HQ a Γ' Δ' ρ n' (cmap_erase m))
     as (a'&?&HA); eauto using indexes_valid_weaken.
-  destruct (HA Γ' Δ'' n'' mA) as (τlr&?&?); clear HA; eauto.
+  destruct (HA Γ' Δ'' n'' mA) as (τlr&?&?); clear HA;
+    eauto 4 using assert_weaken, indexes_valid_weaken.
   { rewrite <-cmap_erase_disjoint_le; auto. }
   destruct τlr as [τ'|]; simplify_option_equality; typed_inversion_all.
   split; [solve_rcred|intros S' p _].
@@ -500,13 +510,14 @@ Proof.
     by (typed_inversion_all; eauto); clear He.
   apply (ax_expr_compose_1 Γ' δ A Q1 _ Δ (DCEltR rs) e ρ n m (inr τ)); auto.
   { esolve_elem_of. }
-  clear dependent m; intros Δ' n' Ω [|v] m ??????; typed_inversion_all.
+  clear dependent m; intros Δ' n' [|v] m ?????; typed_inversion_all.
   apply ax_further_alt.
   intros Δ'' n'' ????? Hframe; inversion_clear Hframe as [mA mf|];
     simplify_equality; simplify_mem_disjoint_hyps.
   destruct (HQ v Γ' Δ' ρ n' (cmap_erase m))
     as (v'&?&HA); eauto using indexes_valid_weaken.
-  destruct (HA Γ' Δ'' n'' mA) as (τlr&?&?); clear HA; eauto.
+  destruct (HA Γ' Δ'' n'' mA) as (τlr&?&?); clear HA;
+    eauto 4 using assert_weaken, indexes_valid_weaken.
   { rewrite <-cmap_erase_disjoint_le; auto. }
   destruct τlr as [|τ']; simplify_option_equality; typed_inversion_all.
   split; [solve_rcred|intros S' p _].
@@ -539,8 +550,8 @@ Proof.
     @sep_union_subseteq_l', @sep_union_subseteq_r'.
   { esolve_elem_of. }
   { esolve_elem_of. }
-  clear dependent m1 m2; intros Δ' n' Ω1 Ω2 [|v1] [|v2] m1 m2
-    ???????????; typed_inversion_all.
+  clear dependent m1 m2.
+  intros Δ' n' [|v1] [|v2] m1 m2 ?????????; typed_inversion_all.
   apply ax_further_alt.
   intros Δ'' n'' ????? Hframe; inversion_clear Hframe as [mA mf|];
     simplify_equality; simplify_mem_disjoint_hyps.
@@ -549,7 +560,8 @@ Proof.
   { rewrite cmap_erase_union.
     exists (cmap_erase m1) (cmap_erase m2); split_ands; auto.
     by rewrite <-!cmap_erase_disjoint_le. }
-  destruct (HA Γ' Δ'' n'' mA) as (?&_&?); clear HA; eauto.
+  destruct (HA Γ' Δ'' n'' mA) as (?&_&?); clear HA;
+    eauto 4 using assert_weaken, indexes_valid_weaken.
   { rewrite <-cmap_erase_disjoint_le; auto. }
   simplify_option_equality; typed_inversion_all.
   split; [solve_rcred|intros S' p _].
@@ -560,6 +572,370 @@ Proof.
   { simpl. by rewrite mem_locks_union by auto. }
   apply ax_done; constructor; eauto using assert_weaken,
     indexes_valid_weaken, val_typed_weaken, val_alter_const_typed.
+Qed.
+Lemma assert_alloc_params P Γ Δ ρ n m mf os vs τs :
+  StackIndep P → ✓ Γ → ✓{Γ,Δ} m → m ⊥ mf → ✓{Δ}* ρ →
+  (Γ,Δ) ⊢* vs :* τs → length os = length vs →
+  Forall_fresh (dom indexset (m ∪ mf)) os →
+  (dom indexset (mem_alloc_list Γ os vs (m ∪ mf)) ∖ dom indexset (m ∪ mf))
+    ∩ dom indexset Δ = ∅ →
+  assert_holds P Γ Δ [] n (cmap_erase m) → ∃ Δ',
+  (**i 1.) *) Δ ⊆ Δ' ∧
+  (**i 2.) *) (∀ Δ'',
+    ✓{Γ,Δ''} (mem_alloc_list Γ os vs m) → Δ ⇒ₘ Δ'' → Δ' ⇒ₘ Δ'') ∧
+  (**i 3.) *) ✓{Δ'}* (zip os τs) ∧
+  (**i 4.) *) ✓{Γ,Δ'} (mem_alloc_list Γ os vs m) ∧
+  (**i 5.) *) mem_alloc_list Γ os vs m ⊥ mf ∧
+  (**i 6.) *) mem_alloc_list Γ os vs (m ∪ mf) = mem_alloc_list Γ os vs m ∪ mf ∧
+  (**i 7.) *) assert_holds
+    (Π imap2_go (λ i v τ,
+      var i ↦{false,perm_full} #freeze true v : τ) (length ρ) vs τs ★ P)%A
+    Γ Δ' (ρ ++ zip os τs) n (cmap_erase (mem_alloc_list Γ os vs m)).
+Proof.
+  intros ??; rewrite <-Forall2_same_length; intros Hm Hmmf Hρ Hvs Hos.
+  revert Δ ρ τs Hm Hρ Hvs; induction Hos as [|o v os vs _ ? IH];
+    intros Δ ρ [|τ τs]; inversion_clear 4; intros Hdom ?; decompose_Forall_hyps.
+  { exists Δ; split_ands; auto. rewrite (right_id_L [] _).
+    rapply (proj2 (left_id (R:=(≡{Γ})) emp (★) P)%A);
+      eauto using stack_indep_spec. }
+  rewrite mem_dom_alloc in Hdom.
+  assert (Δ !! o = None).
+  { apply not_elem_of_dom; clear IH; esolve_elem_of. }
+  assert (Δ ⊆ <[o:=(τ,false)]>Δ) by (by apply insert_subseteq).
+  assert (✓{Γ}(<[o:=(τ,false)]>Δ)) by eauto 3 using mem_alloc_memenv_valid,
+    cmap_valid_memenv_valid, val_typed_type_valid.
+  assert (<[o:=(τ,false)]> Δ ⊢ o : τ) by (by apply mem_alloc_index_typed).
+  destruct (IH (<[o:=(τ,false)]>Δ) (ρ ++ [(o,τ)]) τs)
+    as (Δ'&?&Hleast&?&?&?&->&HP);
+    eauto using assert_weaken, Forall2_impl, val_typed_weaken,
+    cmap_valid_weaken, indexes_valid_weaken; clear IH.
+  { rewrite mem_dom_alloc_list in Hdom |- * by eauto using Forall2_length.
+    rewrite dom_insert_L; esolve_elem_of. }
+  assert (Δ ⊆ Δ') by (by transitivity (<[o:=(τ, false)]> Δ)).
+  assert (o ∉ dom indexset m ∧ o ∉ dom indexset mf) as [??].
+  { by rewrite <-not_elem_of_union, <-cmap_dom_union. }
+  assert (o ∉ dom indexset (mem_alloc_list Γ os vs m)).
+  { by rewrite mem_dom_alloc_list, not_elem_of_union, elem_of_of_list
+      by eauto using Forall2_length. }
+  assert (Δ' ⊢ o : τ)
+    by eauto using memenv_forward_typed, memenv_subseteq_forward.
+  assert (✓{Γ,Δ'} (mem_alloc Γ o false perm_full v (mem_alloc_list Γ os vs m))).
+  { eapply mem_alloc_alive_valid; eauto using val_typed_weaken,
+      memenv_subseteq_alive, mem_alloc_index_alive. }
+  exists Δ'; split_ands; eauto using mem_alloc_disjoint, mem_alloc_union.
+  { intros Δ'' ??; transitivity (<[o:=(τ,false)]> Δ').
+    { by rewrite (insert_id Δ' o (τ,false))
+        by (by apply lookup_weaken with (<[o:=(τ,false)]> Δ); simpl_map). }
+    eapply mem_alloc_forward_least, Hleast;
+      eauto using val_typed_weaken, mem_alloc_valid_inv.
+    destruct (mem_alloc_valid_index_inv Γ Δ'' (mem_alloc_list Γ os vs m) o
+      false perm_full v) as [[??] [??]]; auto; simplify_type_equality.
+    rewrite <-(insert_id Δ'' o (τ,false)) by done.
+    by apply mem_alloc_memenv_compat. }
+  rapply (λ P Q R : assert K, proj1 (associative (R:=(≡{Γ})) (★)%A P Q R));
+    eauto using indexes_valid_weaken.
+  rewrite <-(associative_L (++)), app_length, Nat.add_1_r in HP.
+  destruct (mem_alloc_singleton Γ Δ' (mem_alloc_list Γ os vs m) o
+    false perm_full v τ) as (m'&->&?&?); eauto using val_typed_weaken,
+    memenv_subseteq_alive, mem_alloc_index_alive;
+    simplify_mem_disjoint_hyps.
+  erewrite cmap_erase_union, mem_erase_singleton by eauto.
+  exists m' (cmap_erase (mem_alloc_list Γ os vs m)); split_ands; csimpl;
+    eauto using assert_weaken, mem_alloc_forward.
+  { by rewrite <-cmap_erase_disjoint_le. }
+  eexists (addr_top o τ), (freeze true v); split_ands; auto.
+  * typed_constructor. by rewrite fmap_app,
+      fmap_cons, list_lookup_middle by (by rewrite fmap_length).
+  * by simpl; rewrite list_lookup_middle by done.
+  * typed_constructor; eauto using val_typed_weaken, val_typed_freeze.
+Qed.
+Lemma assert_free_params P Γ Δ ρ n m mf os τs :
+  StackIndep P → ✓ Γ → ✓{Γ,Δ} (m ∪ mf) → m ⊥ mf → ✓{Δ}* ρ → ✓{Δ}* (zip os τs) →
+  assert_holds (Π imap_go (λ i τ, var i ↦{false,perm_full} - : τ)
+    (length ρ) τs ★ P)%A Γ Δ (ρ ++ zip os τs) n (cmap_erase m) →
+  length os = length τs → NoDup os → ∃ Δ',
+  (**i 1.) *) Δ ⇒ₘ Δ' ∧
+  (**i 2.) *) (∀ Δ'', ✓{Γ,Δ''} (foldr mem_free m os) → Δ ⇒ₘ Δ'' → Δ' ⇒ₘ Δ'') ∧
+  (**i 3.) *) ✓{Γ,Δ'} (foldr mem_free m os ∪ mf) ∧
+  (**i 5.) *) foldr mem_free m os ⊥ mf ∧
+  (**i 4.) *) foldr mem_free (m ∪ mf) os = foldr mem_free m os ∪ mf ∧
+  (**i 6.) *) mem_locks (foldr mem_free m os) = mem_locks m ∧
+  (**i 7.) *) assert_holds P Γ Δ' ρ n (cmap_erase (foldr mem_free m os)).
+Proof.
+  intros ?? Hm Hmmf Hρ Hoτs HP; rewrite <-Forall2_same_length; intros Hos.
+  revert Δ ρ m Hρ Hoτs Hm Hmmf HP.
+  induction Hos as [|o τ os τs ? _ IH]; intros Δ ρ m ???? HP;
+    inversion_clear 1; decompose_Forall_hyps; simplify_mem_disjoint_hyps.
+  { rewrite (right_id_L [] _) in HP; exists Δ; split_ands; auto.
+    rapply (proj1 (left_id (R:=(≡{Γ})) emp (★) P)%A); auto. }
+  assert (assert_holds (var (length ρ) ↦{false,perm_full} - : τ ★
+    Π imap_go (λ i τ, (var i ↦{false,perm_full} - : τ)%A) (S (length ρ)) τs ★ P)
+    Γ Δ (ρ ++ (o, τ) :: zip os τs) n (cmap_erase m))
+    as (m1&m2'&?&?&(?&?&v&_&Heval&_&?&?)&?); csimpl in *; [|clear HP].
+  { rapply (λ P Q R : assert K,
+      proj2 (associative (R:=(≡{Γ})) (★)%A P Q R)); auto. }
+  rewrite list_lookup_middle in Heval by done; simplify_option_equality.
+  destruct (cmap_erase_union_inv_l m m1 m2') as (m2&->&?&_&->); auto.
+  simplify_mem_disjoint_hyps.
+  assert (mem_freeable_perm o false m1)
+    by eauto using mem_freeable_perm_singleton.
+  assert (mem_freeable_perm o false (m1 ∪ m2))
+    by eauto using mem_freeable_perm_subseteq, @sep_union_subseteq_l.
+  destruct (IH (alter (prod_map id (λ _, true)) o Δ) (ρ ++ [(o,τ)])
+    (mem_free o (m1 ∪ m2))) as (Δ'&?&Hleast&?&?&?&Hlocks&?);
+    eauto using indexes_valid_weaken, mem_free_forward, mem_free_disjoint.
+  { erewrite <-mem_free_union by eauto; eauto. }
+  { erewrite mem_free_union, cmap_erase_union, mem_free_singleton,
+      sep_left_id, <-(associative_L (++)), app_length, Nat.add_1_r by eauto.
+    eauto 10 using assert_weaken, mem_free_forward. }
+  simplify_mem_disjoint_hyps.
+  assert (Δ ⇒ₘ Δ').
+  { transitivity (alter (prod_map id (λ _, true)) o Δ);
+      auto using mem_free_forward. }
+  rewrite !mem_free_foldr_free; exists Δ'; split_ands; auto.
+  * intros Δ'' Hvalid ?; apply Hleast; auto.
+    assert (∀ τ', Δ'' !! o = Some (τ',false) → False).
+    { intros τ' ?; destruct (mem_free_valid_index_inv Γ Δ''
+        (foldr mem_free (m1 ∪ m2) os) false o); rewrite ?mem_free_foldr_free;
+        auto using mem_freeable_perm_foldr_free.
+      by exists τ'. }
+    rewrite <-(alter_id (prod_map id (λ _, true)) Δ'' o)
+      by (intros [? []] ?; naive_solver); eauto using mem_free_memenv_compat.
+  * by erewrite mem_free_union by eauto.
+  * by erewrite Hlocks, mem_locks_free by eauto.
+  * apply stack_indep_spec with (ρ ++ [(o, τ)]);
+      eauto using indexes_valid_weaken.
+Qed.
+Lemma assert_fun_intro Γ δ (f : funname) Pf τs τ :
+  Γ !! f = Some (τs,τ) →
+  (∀ s c vs,
+    δ !! f = Some s →
+    Γ\ δ ⊨ₛ {{ Π imap2 (λ i v τ,
+                 var i ↦{false,perm_full} #freeze true v : τ) vs τs ★
+               fpre Pf c vs }}
+              s
+            {{ λ v, Π imap (λ i τ, var i ↦{false,perm_full} - : τ) τs ★
+                    fpost Pf c vs v }}) →
+  emp%A ⊆{Γ} assert_fun δ f Pf τs τ.
+Proof.
+  intros ? Hf Γ1 Δ1 ρ n1 m ???? [_ ->].
+  split_ands'; eauto using lookup_fun_weaken.
+  intros Γ2 Δ2 n2 c vs m ?????????.
+  apply ax_further_alt; intros Δ3 n3 ? mf ??? (->&?&?).
+  destruct (funenv_lookup Γ2 Δ2 δ f τs τ) as (s&cmτ&?&_&?&_);
+    eauto using lookup_fun_weaken.
+  assert (✓{Δ2}* ρ) by eauto using indexes_valid_weaken.
+  clear dependent Δ1 n1.
+  split; [solve_rcred|intros S p Hdom].
+  assert (∃ os, Forall_fresh (dom indexset (m ∪ mf)) os ∧
+    length os = length vs ∧
+    S = State [CParams f (zip os (type_of <$> vs))]
+              (Stmt ↘ s) (mem_alloc_list Γ2 os vs (m ∪ mf)))
+    as (os&?&?&->) by (inv_rcstep p; eauto);
+    clear p; simplify_type_equality'.
+  erewrite fmap_type_of by eauto.
+  destruct (assert_alloc_params (fpre Pf c vs) Γ2 Δ3 [] n3 m mf os vs τs)
+    as (Δ4&?&?&?&?&?&->&Hpre); eauto using Forall2_impl, val_typed_weaken,
+    assert_weaken, indexes_valid_weaken.
+  apply mk_ax_next with Δ4 (mem_alloc_list Γ2 os vs m); auto.
+  { constructor; auto. }
+  { eauto using cmap_union_valid_2, cmap_valid_weaken. }
+  { intros; simplify_mem_disjoint_hyps; eauto. }
+  destruct (funenv_lookup Γ2 Δ2 δ f τs τ) as (?&τlr&?&?&?&?&?&?);
+    eauto using lookup_fun_weaken; simplify_equality.
+  assert (length os = length τs).
+  { erewrite <-(Forall2_length _ _ τs) by eauto; lia. }
+  assert (NoDup os)
+    by (by apply Forall_fresh_NoDup with (dom indexset (m ∪ mf))).
+  eapply ax_compose_cons with ax_disjoint_cond _; eauto.
+  { eapply Hf, Hpre; eauto using funenv_valid_weaken.
+    * by transitivity Γ1.
+    * assert (Forall_fresh (dom indexset m) os).
+      { eapply Forall_fresh_subseteq; eauto.
+        rewrite cmap_dom_union; solve_elem_of. }
+      by erewrite mem_locks_alloc_list by eauto.
+    * simpl; rewrite snd_zip by lia; eauto using stmt_typed_weaken. }
+  clear dependent m mf; intros Δ5 n4 ? m; destruct 1; intros.
+  apply ax_further_alt; intros Δ6 n5 ? mf ??? (->&?&?).
+  split; [solve_rcred|intros S p _].
+  assert (∃ v, S = State [] (Return f v) (foldr mem_free (m ∪ mf) os) ∧
+    assert_holds (Π imap (λ i τ, (var i ↦{false,perm_full} - : τ)%A) τs
+      ★ fpost Pf c vs v) Γ2 Δ5 (zip os τs) n4 (cmap_erase m) ∧
+    (Γ2,Δ5) ⊢ v : τ) as (v&->&?&?).
+  { inv_rcstep; typed_inversion_all;
+      match goal with H : rettype_match _ _ |- _ => inversion H; subst end;
+      eexists; split_ands; rewrite ?fst_zip by auto; eauto. }
+  clear dependent p d.
+  destruct (assert_free_params (fpost Pf c vs v) Γ2 Δ6 [] n5 m mf os τs)
+    as (Δ7&?&?&?&?&->&?&?); eauto using assert_weaken, indexes_valid_weaken.
+  apply mk_ax_next with Δ7 (foldr mem_free m os); auto.
+  { constructor; auto. }
+  { intros; simplify_mem_disjoint_hyps; eauto. }
+  apply ax_done; constructor; eauto using val_typed_weaken with congruence.
+Qed.
+Lemma ax_call {vn} Γ δ A Pf P Q Ps Qs R e (es : vec (expr K) vn) τs τ c :
+  (∀ v vs,
+    (A ★ Q (inr v) ★ Π vzip_with (λ Q v, Q (inr v)) Qs vs)%A ⊆{Γ} (∃ f,
+      ⌜ v = ptrV (FunPtr f τs τ) ⌝ ★ 
+      ▷ (assert_fun δ f Pf τs τ) ★ fpre Pf c vs ★
+      (∀ vret, fpost Pf c vs vret -★ (A ★ R (inr vret))))%A) →
+  Γ\ δ \ A ⊨ₑ {{ P }} e {{ λ ν, (Q ν) ◊ }} →
+  (∀ i, Γ\ δ\ A ⊨ₑ {{ Ps !!! i }} es !!! i {{ λ ν, ((Qs !!! i) ν) ◊ }}) →
+  Γ\ δ \ A ⊨ₑ {{ P ★ Π Ps }} call e @ es {{ R }}.
+Proof.
+  intros HQ Hax1 Hax2 Γ' Δ n ρ m τlr ????? He ??? HP.
+  assert (∃ τ (τs : vec _ vn), τlr = inr τ ∧
+    (Γ',Δ,ρ.*2) ⊢ e : inr ((τs ~> τ).*) ∧
+    ∀ i, (Γ',Δ,ρ.*2) ⊢ es !!! i : inr (τs !!! i))
+    as (τ'&τs'&->&?&?); [|clear He].
+  { assert (∃ τ τs, τlr = inr τ ∧ (Γ',Δ,ρ.*2) ⊢ e : inr ((τs ~> τ).*) ∧
+      (Γ',Δ,ρ.*2) ⊢* es :* inr <$> τs) as (τ'&τs'&->&?&Hes)
+      by (typed_inversion_all; eauto).
+    assert (vn = length τs') by (by erewrite <-fmap_length,
+      <-Forall2_length, vec_to_list_length by eauto); subst vn.
+    exists τ' (list_to_vec τs'). rewrite ?vec_to_list_of_list.
+    by rewrite Forall2_fmap_r, <-(vec_to_list_of_list τs'),
+      Forall2_vlookup in Hes. }
+  destruct HP as (m1'&m2&Hm&Hm'&?&HPs).
+  destruct (cmap_erase_union_inv_r m m1' m2)
+    as (m1&->&?&->&?); simplify_mem_disjoint_hyps; auto; clear Hm Hm'.
+  rewrite assert_Forall_holds_vec in HPs; destruct HPs as (ms&->&?&?).
+  repeat match goal with
+    | _ => progress simpl in *
+    | H : mem_locks (_ ∪ _) = ∅ |- _ => rewrite mem_locks_union in H by auto
+    | H : mem_locks (⋃ _) = ∅ |- _ => rewrite mem_locks_union_list in H by auto
+    | H : ✓{_} (⋃ _) |- _ =>
+       rewrite <-cmap_union_list_valid, Forall_vlookup in H by eauto
+    | H : _ ∪ _ = ∅ |- _ => apply empty_union_L in H; destruct H
+    | H : ⋃ _ = ∅ |- _ =>
+       rewrite empty_union_list_L, Forall_fmap, Forall_vlookup in H
+    end.
+  apply (ax_expr_compose Γ' δ A ((λ ν, Q ν ◊)%A ::: vmap (λ Q ν, Q ν ◊)%A Qs) R
+    Δ (DCCall vn) (e ::: es) ρ n
+    (m1 ::: ms) (inr ((τs' ~> τ').*) ::: vmap inr τs')); auto.
+  { intros i; inv_fin i; eauto. }
+  { intros i; inv_fin i; esolve_elem_of. }
+  { intros i; inv_fin i; simpl.
+    { eauto using ax_expr_invariant_weaken, @sep_union_subseteq_l'. }
+    intros i; rewrite vlookup_map; eapply Hax2; eauto.
+    * by rewrite vlookup_map.
+    * eapply ax_expr_invariant_weaken; eauto.
+      by apply sep_union_subseteq_r_transitive, (sep_subseteq_lookup ms).
+    * by rewrite cmap_erased_spec
+        by eauto using cmap_erased_subseteq, (sep_subseteq_lookup ms). }
+  clear dependent m1 ms e es P Ps; intros Δ' n' νs ms.
+  inv_vec νs; intros ν νs; inv_vec ms; intros m ms.
+  intros ? Hms ?? Hνs HQs;
+    repeat match goal with
+    | H : ∀ i : fin (S _), _ |- _ =>
+       pose proof (H 0%fin); specialize (λ i, H (FS i)); simpl in *
+    | H : assert_holds _ _ _ _ _ _ |- _ => rewrite assert_unlock_spec in H
+    end.
+  destruct ν as [|v]; typed_inversion_all.
+  assert (∃ vs, νs = vmap inr vs ∧ (Γ',Δ') ⊢* vs :* τs') as (vs&->&Hvs).
+  { revert Hνs; clear; induction νs as [|ν ? νs IH].
+    { inv_vec τs'; eexists [#]; simpl; auto. }
+    inv_vec τs'; intros τ τs Hi; destruct (IH τs (λ i, Hi (FS i))) as (vs&->&?).
+    specialize (Hi 0%fin); typed_inversion_all; eexists (_:::_); simpl; eauto. }
+  clear Hνs.
+  rewrite vec_to_list_zip_with, vec_to_list_map, zip_with_fmap_r.
+  rewrite <-(zip_with_fmap_l (λ Ω v, #{Ω} v)%E mem_locks).
+  apply ax_further_alt.
+  intros Δ'' n'' ????? Hframe; inversion_clear Hframe as [mA mf ?????? HmA|];
+    simplify_equality; simplify_mem_disjoint_hyps.
+  destruct (HQ v vs Γ' Δ'' ρ (S n'')
+    (cmap_erase (mem_unlock_all (m ∪ ⋃ ms ∪ mA))))
+    as (f&?&?&Hm&_&[-> ->]&?&?&->&_&Hf&m''&mf2&->&?&?&Hpost); clear HQ;
+    eauto using indexes_valid_weaken, mem_unlock_all_valid.
+  { assert (⊥ (mA :: cmap_erase m :: cmap_erase <$> vec_to_list ms)).
+    { rewrite <-cmap_erase_disjoint_le, <-cmap_erase_disjoint_list_le; auto. }
+    rewrite (sep_commutative _ mA), mem_erase_unlock_all by auto.
+    rewrite !cmap_erase_union,
+      cmap_erase_union_list, (cmap_erased_spec mA) by auto.
+    rewrite !mem_unlock_all_union,
+      mem_unlock_all_union_list, (mem_unlock_all_empty_locks mA) by auto.
+    assert (⊥ (mA :: mem_unlock_all (cmap_erase m) ::
+      mem_unlock_all <$> cmap_erase <$> vec_to_list ms)) by
+      by rewrite <-mem_unlock_all_disjoint_le,<-mem_unlock_all_disjoint_list_le.
+    eexists mA, _; split_ands; auto.
+    eexists _, _; split_ands;
+      eauto using assert_weaken, indexes_valid_weaken, mem_unlock_all_valid.
+    apply assert_Forall_holds_2; auto.
+    rewrite <-!vec_to_list_map, Forall2_vlookup; intros i; specialize (HQs i).
+    rewrite !vlookup_map, vlookup_zip_with.
+    rewrite !vlookup_map, assert_unlock_spec in HQs; simpl in *.
+    eauto using assert_weaken, indexes_valid_weaken, mem_unlock_all_valid. }
+  destruct (Hf n'') as (->&?&Hf'); clear Hf; auto.
+  rewrite !sep_left_id in Hm by auto; typed_inversion_all.
+  assert (⊥ [mem_unlock_all (m ∪ ⋃ ms ∪ mA); mf])
+    by (rewrite <-mem_unlock_all_disjoint_le; auto).
+  destruct (cmap_erase_union_inv_r (mem_unlock_all (m ∪ ⋃ ms ∪ mA)) m'' mf2)
+    as (m'&Hm'&?&->&?); auto.
+  assert (mem_locks m' = ∅ ∧ mem_locks mf2 = ∅) as [??].
+  { rewrite <-empty_union_L, <-mem_locks_union, <-Hm' by auto.
+    by rewrite mem_locks_unlock_all. }
+  assert (✓{Γ',Δ''} (mem_unlock_all (m ∪ ⋃ ms ∪ mA)))
+    by eauto using mem_unlock_all_valid.
+  assert (✓{Γ',Δ''} m' ∧ ✓{Γ',Δ''} mf2) as [??].
+    by (rewrite <-cmap_union_valid, <-Hm' by auto; auto).
+  assert (length (mem_locks <$> vec_to_list ms) = length vs).
+  { rewrite fmap_length; apply vec_to_list_same_length. }
+  split; [solve_rcred|intros ? p _].
+  apply (rcstep_expr_call_inv _ _ _ _ _ _ _ _ _ _ _ _ p); auto; clear p.
+  assert (mem_locks (m ∪ ⋃ ms ∪ mA) =
+    mem_locks m ∪ ⋃ (mem_locks <$> vec_to_list ms)).
+  { rewrite !mem_locks_union, mem_locks_union_list by auto.
+    by rewrite HmA, (right_id_L _ _). }
+  rewrite <-sep_associative, (sep_commutative mf), sep_associative by auto.
+  rewrite mem_unlock_union, <-mem_unlock_all_spec_alt
+    by eauto using (reflexive_eq (R:=(⊆) : relation lockset)), eq_sym.
+  apply mk_ax_next with Δ'' (mem_unlock_all (m ∪ ⋃ ms ∪ mA)); auto.
+  { apply ax_unframe_expr_to_fun with (mem_unlock_all (m ∪ ⋃ ms)); auto.
+    * by rewrite mem_unlock_all_union, (mem_unlock_all_empty_locks mA) by auto.
+    * rewrite mem_unlock_all_union, (mem_unlock_all_empty_locks mA) by auto.
+      by rewrite <-!sep_associative, (sep_commutative mA)
+        by (rewrite <-?mem_unlock_all_disjoint_le; auto).
+    * rewrite <-mem_unlock_all_disjoint_le; auto. }
+  rewrite Hm'; clear dependent m ms mA mf S'.
+  eapply ax_compose_cons with ax_disjoint_cond
+    (ax_fun_post f τ' (λ v, fpost Pf c vs v ★ assert_eq_mem mf2)%A); auto.
+  { apply ax_frame with ax_disjoint_cond (ax_fun_post f τ' (fpost Pf c vs));
+      auto using ax_disjoint_cond_frame_diagram.
+    apply Hf'; eauto using funenv_valid_weaken, Forall2_impl, val_typed_weaken.
+    { eapply stack_indep_spec with ρ;
+        eauto using assert_weaken, indexes_valid_weaken. }
+    intros Δ''' n''' ? m'' ?????; destruct 1; constructor; auto.
+    * by rewrite mem_locks_union, empty_union_L by auto.
+    * rewrite cmap_erase_union, (cmap_erased_spec mf2) by auto.
+      exists (cmap_erase m) mf2; split_ands; try done.
+      by rewrite <-cmap_erase_disjoint_le. }
+  clear dependent m' Hf'.
+  intros Δ''' n''' m'; destruct 1 as [v m''' ?? (m''&?&?&?&?&Hmf)]; intros.
+  repeat red in Hmf; subst. 
+  destruct (cmap_erase_union_inv_r m''' m'' mf2) as (m&->&?&->&?); auto.
+  apply ax_further_alt; intros Δ'''' n'''';
+    destruct 4; simplify_equality'; simplify_mem_disjoint_hyps.
+  split; [solve_rcred|intros S' p _; inv_rcstep p].
+  destruct (Hpost v Γ' Δ'''' (S n'''') (cmap_erase m))
+    as (mA&m''&?&?&?&?); auto.
+  { eapply stack_indep_spec with [];
+      eauto using assert_weaken, indexes_valid_weaken. }
+  destruct (cmap_erase_union_inv_l (m ∪ mf2) mA m'')
+    as (m'&Hm'&?&?&->); auto.
+  { by rewrite cmap_erase_union, (cmap_erased_spec mf2) by auto. }
+  assert (⊥ [mA ∪ m'; mf]) by (rewrite <-Hm'; auto).
+  assert (mem_locks mA = ∅ ∧ mem_locks m' = ∅) as [??].
+  { by rewrite <-empty_union_L, <-mem_locks_union, <-Hm' by auto. }
+  assert (✓{Γ',Δ''''} mA ∧ ✓{Γ',Δ''''} m') as [??].
+  { rewrite <-cmap_union_valid, <-Hm' by auto; auto. }
+  assert (mem_locks mA = ∅ ∧ mem_locks m' = ∅) as [??].
+  { by rewrite <-empty_union_L, <-mem_locks_union, <-Hm' by auto. }
+  rewrite Hm', <-sep_associative, (sep_commutative mA) by auto.
+  apply mk_ax_next with Δ'''' m'; simpl; auto.
+  { apply ax_unframe_fun_to_expr with mA; auto. }
+  { apply subseteq_empty. }
+  apply ax_done; constructor; eauto 7 using val_typed_weaken,
+    assert_weaken, indexes_valid_weaken.
 Qed.
 Lemma ax_alloc Γ δ A P Q1 Q2 e τ :
   (∀ o vb,
@@ -579,7 +955,7 @@ Proof.
     (DCAlloc τ) e ρ n m (inr (intT τi))); auto.
   { esolve_elem_of. }
   clear dependent m.
-  intros Δ' n' Ω [|[vb| | | |]] m ??????; typed_inversion_all.
+  intros Δ' n' [|[vb| | | |]] m ?????; typed_inversion_all.
   destruct (HQ (fresh ∅) vb Γ' Δ' ρ n' (cmap_erase m)) as
     (na&τi'&?&?&Hm&Hm'&[[-> ?] ->]&[_ Hfail]); eauto using indexes_valid_weaken;
     typed_inversion_all.
@@ -599,7 +975,7 @@ Proof.
     apply ax_done; constructor; eauto 10 using type_valid_ptr_type_valid.
     assert (⊥ [∅; cmap_erase m]).
     { rewrite <-cmap_erase_disjoint_le; auto. }
-    rewrite <-(sep_left_id (cmap_erase m)) by auto; eapply Hfail; eauto. }
+    rewrite <-(sep_left_id (cmap_erase m)) by auto; by eapply Hfail; eauto. }
   assert (Δ'' !! o = None); [|clear Hdom].
   { rewrite mem_dom_alloc in Hdom. apply not_elem_of_dom; esolve_elem_of. }
   rewrite <-sep_associative, cmap_dom_union,
@@ -616,7 +992,7 @@ Proof.
   { simpl. by erewrite (mem_locks_alloc _ Δ'') by eauto. }
   apply ax_done; constructor; eauto 8 using addr_top_array_typed,
     mem_alloc_index_typed, (mem_locks_alloc _ Δ'').
-  destruct (mem_alloc_singleton Γ' Δ'' m o true perm_full
+  destruct (mem_alloc_singleton_alt Γ' Δ'' m o true perm_full
     (val_new Γ' (τ.[Z.to_nat na])) (τ.[Z.to_nat na]))
     as (m'&Hm'&?&?); auto using val_new_frozen.
   rewrite Hm' in *; simplify_mem_disjoint_hyps; clear Hm'.
@@ -627,7 +1003,8 @@ Proof.
   eapply HQ2; eauto using mem_alloc_forward, indexes_valid_weaken; clear HQ2.
   { by eapply mem_singleton_valid;
       eauto using mem_alloc_memenv_valid, mem_alloc_index_alive. }
-  { eauto using mem_alloc_orig_valid. }
+  { eauto using cmap_valid_weaken,
+      (insert_subseteq Δ''), mem_alloc_memenv_valid. }
   { by rewrite <-cmap_erase_disjoint_le. }
   eexists _, (addr_top o (τ.[Z.to_nat na'])), (val_new Γ' (τ.[Z.to_nat na']));
     split_ands; eauto using addr_top_typed, mem_alloc_index_typed.
@@ -646,7 +1023,7 @@ Proof.
     by (typed_inversion_all; eauto); clear He.
   apply (ax_expr_compose_1 Γ' δ A Q1 _ Δ DCFree e ρ n m (inl τ')); auto.
   { esolve_elem_of. }
-  clear dependent m; intros Δ' n' Ω [a|] m ??????; typed_inversion_all.
+  clear dependent m; intros Δ' n' [a|] m ?????; typed_inversion_all.
   destruct (HQ a Γ' Δ' ρ n' (cmap_erase m))
     as (na&?&?&Hm'&?&[Ha' ->]&m1&m2'&?&?&(ν&a'&v&_&?&?&?&?)&?);
     eauto using indexes_valid_weaken.
@@ -693,13 +1070,14 @@ Proof.
     as (τ&?&?) by (typed_inversion_all; eauto); clear He.
   apply (ax_expr_compose_1 Γ' δ A Q1 _ Δ (DCUnOp op) e ρ n m (inr τ)); auto.
   { esolve_elem_of. }
-  clear dependent m. intros Δ' n' Ω [a|] m ??????; typed_inversion_all.
+  clear dependent m. intros Δ' n' [a|] m ?????; typed_inversion_all.
   apply ax_further_alt.
   intros Δ'' n'' ????? Hframe; inversion_clear Hframe as [mA mf|];
     simplify_equality; simplify_mem_disjoint_hyps.
   destruct (HQ v Γ' Δ' ρ n' (cmap_erase m))
     as (v'&?&HA); eauto using indexes_valid_weaken.
-  destruct (HA Γ' Δ'' n'' mA) as (?&_&?); clear HA; eauto.
+  destruct (HA Γ' Δ'' n'' mA) as (?&_&?); clear HA;
+    eauto 4 using assert_weaken, indexes_valid_weaken.
   { rewrite <-cmap_erase_disjoint_le; auto. }
   simplify_option_equality.
   assert (val_unop_ok (m ∪ mf ∪ mA) op v).
@@ -737,8 +1115,8 @@ Proof.
     @sep_union_subseteq_l', @sep_union_subseteq_r'.
   { esolve_elem_of. }
   { esolve_elem_of. }
-  clear dependent m1 m2; intros Δ' n' Ω1 Ω2 [|v1] [|v2] m1 m2
-    ???????????; typed_inversion_all.
+  clear dependent m1 m2; intros Δ' n' [|v1] [|v2] m1 m2
+    ?????????; typed_inversion_all.
   apply ax_further_alt.
   intros Δ'' n'' ????? Hframe; inversion_clear Hframe as [mA mf|];
     simplify_equality; simplify_mem_disjoint_hyps.
@@ -747,7 +1125,8 @@ Proof.
   { rewrite cmap_erase_union.
     exists (cmap_erase m1) (cmap_erase m2); split_ands; auto.
     by rewrite <-!cmap_erase_disjoint_le. }
-  destruct (HA Γ' Δ'' n'' mA) as (?&_&?); clear HA; eauto.
+  destruct (HA Γ' Δ'' n'' mA) as (?&_&?); clear HA;
+    eauto 4 using assert_weaken, indexes_valid_weaken.
   { rewrite <-cmap_erase_disjoint_le; auto. }
   simplify_option_equality.
   assert (val_binop_ok Γ' (m1 ∪ m2 ∪ mf ∪ mA) op v1 v2).
@@ -775,13 +1154,14 @@ Proof.
     as (τ&?&?&?&->) by (typed_inversion_all; eauto); clear He.
   apply (ax_expr_compose_1 Γ' δ A Q1 _ Δ (DCCast σ) e ρ n m (inr τ)); auto.
   { esolve_elem_of. }
-  clear dependent m. intros Δ' n' Ω [a|] m ??????; typed_inversion_all.
+  clear dependent m. intros Δ' n' [a|] m ?????; typed_inversion_all.
   apply ax_further_alt.
   intros Δ'' n'' ????? Hframe; inversion_clear Hframe as [mA mf|];
     simplify_equality; simplify_mem_disjoint_hyps.
   destruct (HQ v Γ' Δ' ρ n' (cmap_erase m))
     as (v'&?&HA); eauto using indexes_valid_weaken.
-  destruct (HA Γ' Δ'' n'' mA) as (?&_&?); clear HA; eauto.
+  destruct (HA Γ' Δ'' n'' mA) as (?&_&?); clear HA;
+    eauto 4 using assert_weaken, indexes_valid_weaken.
   { rewrite <-cmap_erase_disjoint_le; auto. }
   simplify_option_equality.
   assert (val_cast_ok Γ' (m ∪ mf ∪ mA) (TType σ) v).
@@ -815,7 +1195,7 @@ Proof.
   { esolve_elem_of. }
   { esolve_elem_of. }
   clear dependent m;
-    intros Δ' n' Ω [|[vb| | | |]] m ??????; typed_inversion_all.
+    intros Δ' n' [|[vb| | | |]] m ?????; typed_inversion_all.
   apply ax_further_alt.
   intros Δ'' n'' ????? Hframe; inversion_clear Hframe as [mA mf|];
     simplify_equality; simplify_mem_disjoint_hyps.
@@ -824,8 +1204,8 @@ Proof.
       by (rewrite <-cmap_erase_disjoint_le; auto).
     destruct (HP' vb Γ' Δ'' ρ n'' (mA ∪ cmap_erase m)) as (?&?&?&?);
       simpl; eauto using indexes_valid_weaken.
-    { exists mA (cmap_erase m); split_ands; auto.
-      eauto using assert_weaken, indexes_valid_weaken. }
+    { exists mA (cmap_erase m); split_ands;
+        eauto 4 using assert_weaken, indexes_valid_weaken. }
     simplify_option_equality.
     eapply base_val_branchable_weaken with (mA ∪ cmap_erase m); eauto.
     intros; eapply cmap_subseteq_index_alive; eauto.
@@ -846,7 +1226,7 @@ Proof.
     apply Hax1; rewrite ?mem_erase_unlock_all;
       eauto 8 using mem_unlock_all_valid, indexes_valid_weaken,
       mem_locks_unlock_all, expr_typed_weaken, funenv_valid_weaken.
-    + exists mA; split_ands; eauto.
+    + exists mA; eauto 8 using assert_weaken, indexes_valid_weaken.
     + eapply HP1; eauto using indexes_valid_weaken, assert_weaken.
   * rewrite !mem_unlock_union, <-mem_unlock_all_spec
       by (rewrite ?mem_locks_union by auto; solve_elem_of).
@@ -857,7 +1237,7 @@ Proof.
     apply Hax2; rewrite ?mem_erase_unlock_all;
       eauto 8 using mem_unlock_all_valid, indexes_valid_weaken,
       mem_locks_unlock_all, expr_typed_weaken, funenv_valid_weaken.
-    + exists mA; split_ands; eauto.
+    + exists mA; eauto 8 using indexes_valid_weaken, assert_weaken.
     + eapply HP2; eauto using indexes_valid_weaken, assert_weaken.
   * destruct (decide (base_val_is_0 vb)); exfalso; eauto with cstep.
 Qed.
@@ -873,7 +1253,8 @@ Proof.
   apply (ax_expr_compose_1 Γ' δ A
     (λ _, P' ◊)%A _ Δ (DCComma e2) e1 ρ n m τlr1); auto.
   { esolve_elem_of. }
-  clear dependent m; intros Δ' n' Ω ν m ??????; simplify_equality'.
+  clear dependent m; intros Δ' n' ν m;
+    rewrite assert_unlock_spec; intros ?????; simplify_equality'.
   apply ax_further; [intros; solve_rcred|].
   intros Δ'' n'' ?? S' ??? Hframe p _; inversion_clear Hframe as [mA mf|];
     simplify_equality; simplify_mem_disjoint_hyps.
@@ -889,6 +1270,6 @@ Proof.
   apply Hax2; rewrite ?mem_erase_unlock_all;
     eauto 7 using mem_unlock_all_valid, indexes_valid_weaken,
     mem_locks_unlock_all, expr_typed_weaken, assert_weaken, funenv_valid_weaken.
-  exists mA; split_ands; eauto.
+  exists mA; eauto 8 using indexes_valid_weaken, assert_weaken.
 Qed.
 End axiomatic_expressions.
